---
layout: post
title: The Ramsey Model (p1)
published: true
date: 2022-2-20
categories: [literature]
tags: [ramsey]
series: "Ramsey"
---

This note compiles some essential techniques in solving the Ramsey model. At the moment, only solutions for households are included. I will consider more extensions at a later time. For economic intuitive intepretations, see the free book [Campante, Filipe, Sturzenegger, Federico and Velasco, AndrÃ©s  (2021) Advanced macroeconomics: an easy guide. LSE Press, London, UK. ISBN 9781909890688](http://eprints.lse.ac.uk/112475/).
	
In this neoclassical growth model, we assume there is one representative household maximizing her utility function at each point in time with forward-looking ability. She cares about future consumption with some discount weights. Her life-time utility function can be represented as follows. In the discrete-time version, one can use inter-temporal Lagrangian or Bellman's dynamic programming to solve the problem. In the continuous-time version, Lagrangian is also possible and then shorthanded with Hamiltonian. In both cases, the household is assumed to live forever.

Part 1 deals with the discrete-time version.

{% include series.html %}

## Discrete Time

Let us deal with the discrete version first.

### Household's Problem

The life-time utility function is:

$$
    U_t = u_0 + \frac{u_1}{1+\rho} + \frac{u_2}{(1+\rho)^2} + \dots = \sum_{t=0}^{\infty} \frac{u_t}{(1+\rho)^t}
$$

where $u_t = u(c_t)$, so that utility at time $t$ derived from consumption $c_t$ at time $t$. To simplify the notation, denote the discount factor as $\beta \equiv \frac{1}{1+\rho}$ so that the household obtains an objective function:

$$
    \max_{c_t} U_t = \sum_{t=0}^{\infty} \beta^t u(c_t) \ \ (1)
$$

The budget constraint:

$$
     c_t + i_t = f(k_t)              \\
     k_{t+1} = i_t + (1- \delta) k_t \\
     k_0 > 0                         
$$

where $i$ is investment, which will be carried over to form the next period's capital stock. Capital depreciates with the rate of $\delta$.

Combining the above equations gives:

$$             
    c_t = f(k_t) - k_{t+1} + (1-\delta)k_t \ \ (2)
$$

One can rearrange to see the increase in capital stock over time:

$$
    k_{t+1} - k_t = f(k_t) - \delta k_t - c_t 
$$

which will help us find the budget constraint for the continuous time version.

### The Lagrangian Method

The Lagrangian:

$$
    \mathcal{L} = \sum_{t=0}^{\infty} \beta^t u(c_t) + \sum_{t=0}^{\infty} \lambda_t \left[ f(k_t) + (1- \delta) k_t - k_{t+1} - c_t \right]
$$	

Grouping all the summation and rewrite the Lagrangian:
$$
    \mathcal{L} = \sum_{t=0}^{\infty} \left[ \beta^t u(c_t) + \lambda_t \left( f(k_t) + (1- \delta)k_t - k_{t+1} - c_t \right) \right]
$$

The term inside the sum should be optimized in each point in time. The modified Lagrangian:
$$
    \triangle = \beta^t u(c_t) + \lambda_t \left( f(k_t) + (1- \delta) k_t - k_{t+1} - c_t \right)
$$

FOC: (Note that $k_{t+1}$ appears twice at time $t$ and $t+1$)

$$
      (c_t): \frac{\partial \triangle}{\partial c_t} = \beta^t u'(c_t) - \lambda_t = 0    \ \ (3)                                               \\
      (k_{t+1}): \frac{\partial \triangle}{\partial k_{t+1}} = -\lambda_t + \lambda_{t+1} \left[ f'(k_{t+1}) + (1-\delta) \right] = 0 \ \ (4)
$$

By virtue of Eq. (3), we see that:

$$
    \beta^{t+1}u'(c_{t+1}) = \lambda_{t+1}
$$

Plugging back to Eq. (4) and rearranging give us the Euler equation:

$$
    \frac{u'(c_t)}{u'(c_{t+1})} = \beta \left[ f'(k_{t+1}) + (1-\delta) \right]
$$

Consider the utility function $u(c_t) = \ln(c_t)$, we have:

$$
    \frac{c_{t+1}}{c_t} = \beta \left[f'(k_{t+1}) + (1-\delta)\right]
$$

In the steady-state, $c_{t+1} = c_t = \bar{c}$ and $k_{t+1} = k_t = \bar{k}$.  

Provided with a functional form of the production function $f(k)$, one can find the steady-state values of $\bar{c}, \bar{k}$ and then use backward induction to figure out the dynamics from a given $k_0$.

### Dynamic Programming (Bellman Equation)

Another method of solving is to use the Bellman equation. First, we replace $c_t$ in Eq. (2) with Eq. (3). The objective function becomes:

$$
    \max_{k_{t+1}} U_t = \sum_{t=0}^{\infty} \beta^t u \left(f(k_t) + (1-\delta)k_t - k_{t+1} \right)
$$

Imagine we are at time $t=0$, the problem is:

$$
    \max \sum_{t=0}^{\infty} \beta^t u \left(f(k_t) + (1-\delta)k_t - k_{t+1} \right) \equiv L_0
$$

In the next period $t=1$:

$$
    \max \sum_{t=1}^{\infty} \beta^t u \left(f(k_t) + (1-\delta)k_t - k_{t+1} \right) \equiv L_1
$$

Although the 2 problems look almost identical, there are 2 fundamental differences. First, at $t=0$, we know $k_0$ but do not know $k_1$, we maximize and then find $k_1$, whereas at $t=1$, we already know $k_1$ (and of course $k_0$). Second, at $t=1$, the terms have been shifted 1 period forward, which means the future maximization problem must be discounted by $\beta$. 

Thus, we can nest tomorrow's problem into today's problem as follows:

$$
    L_0 = \max \left[ u(f(k_0) + (1-\delta)k_0 - k_1) + L_1 \right]
$$

At $t=0$, $k_0$ is the key to determine $L_0$. At $t=1$, $k_1$ becomes the key to determine $L_1$. By valuating $L$ associated with the known $k$ at that time, we arrive at:

$$
    L(k_0) =  \max \left[ u(f(k_0) + (1-\delta)k_0 - k_1) + \beta L(k_1) \right]
$$

We can rewrite this expression into a Bellman equation, with $V(k)$ be the Value function. Also, the optimal solution must be true for any time $t$, so we generalize it as follows.

$$
    V(k_t) =  \max \left[ u(f(k_t) + (1-\delta)k_t - k_{t+1}) + \beta V(k_{t+1}) \right] \ \ (5)
$$

FOC with respect to $k_{t+1}$:

$$
    \frac{\partial V(k_t)}{\partial k_{t+1}} = - u'(f(k_t) + (1-\delta) - k_{t+1}) + \beta \frac{\partial V(k_{t+1})}{\partial k_{t+1}} = 0
$$

To find $\frac{\partial V(k_{t+1})}{\partial k_{t+1}}$, first take the derivatives of Eq. (5) wrt to $k_t$:

$$
    \frac{\partial V(k_t)}{\partial k_t} = (f'(k_t) + 1 - \delta) u'(f(k_t) + (1-\delta)k_t - k_{t+1})
$$

which implies:

$$
    \frac{\partial V(k_{t+1})}{\partial k_{t+1}} = (f'(k_{t+1}) + 1 - \delta) u'(f(k_{t+1}) + (1-\delta)k_{t+1} - k_{t+2})
$$

Plugging back to the FOC to obtain:

$$
    u'(\underbrace{f(k_t) + (1-\delta) - k_{t+1}}_{c_t}) = \beta [f'(k_{t+1}) + (1 - \delta)] u'(\underbrace{f(k_{t+1}) + (1-\delta)k_{t+1} - k_{t+2}}_{c_{t+1}})
$$

Rearranging gives us the Euler equation:

$$
    \frac{u'(c_t)}{u'(c_{t+1})} = \beta \left[f'(k_{t+1}) + (1-\delta) \right]
$$

For technical reasons, the transversality condition is needed	 (which is seen better at the continuous time section):

$$
    \lim_{t\to\infty} \beta^t u'(c_t)k_{t+1} = 0
$$

An intuitive explanation can be found [here](https://www.rieb.kobe-u.ac.jp/academic/ra/dp/English/dp180.pdf). For now, so long as $\beta < 1$, this condition is always satisfied.

------
I own a spiritual debt to [Constantin Burgi](http://www.musikbase.net/cburgi/index.html) and his lectures on [Youtube](https://www.youtube.com/channel/UCSPwROlKXYWaQCI5kcmTCjw/videos). This note stems from lectures by Prof. [Kitagawa Akiomi](http://www2.econ.tohoku.ac.jp/~kitagawa/) and [Tomoaki Kotera](https://sites.google.com/site/tomoakikotera39/home/research) at Tohoku University.